verif/verif_findindex.v
@@ -1,0 +1,44 @@
+(** * verif_findindex.v : Correctness proof of findChildIndex and findRecordIndex *)
+
+Require Import VST.floyd.proofauto.
+Require Import VST.floyd.library.
+Require Import relation_mem.
+Instance CompSpecs : compspecs. make_compspecs prog. Defined.
+Definition Vprog : varspecs. mk_varspecs prog. Defined.
+
+Require Import VST.msl.wand_frame.
+Require Import VST.msl.iter_sepcon.
+Require Import VST.floyd.reassoc_seq.
+Require Import VST.floyd.field_at_wand.
+Require Import FunInd.
+Require Import btrees.
+Require Import btrees_sep.
+Require Import btrees_spec.
+Require Import index.
+
+Lemma body_findChildIndex: semax_body Vprog Gprog f_findChildIndex findChildIndex_spec.
+Proof.
+  start_function.
+  forward.                      (* i=0 *)
+  forward_if (PROP() LOCAL (temp _i (Vint (Int.repr 0)); temp _length (Vint (Int.repr (Z.of_nat (numKeys_le le)))); temp _key (Vint (Int.repr key)); temp _entries p)  SEP (le_iter_sepcon le)).
+  - forward.                    (* skip *)
+    entailer!. admit.           (* why is valid_pointer gone from the postcondition? *)
+  - contradiction.
+  - forward_if(PROP ( ) LOCAL (temp _i (Vint (Int.repr 0)); temp _length (Vint (Int.repr (Z.of_nat (numKeys_le le)))); temp _key (Vint (Int.repr key)); temp _entries p)  SEP (le_iter_sepcon le)).
+    + forward.                  (* skip *)
+      entailer!.
+    + destruct le. contradiction. simpl in H1.
+      clear -H1. admit.
+      (* there's a contradiction in h1. rep_omega takes forever *)
+    + destruct le as [|e le']; try contradiction.
+      simpl.
+      (* _entries+(0) should be e *)
+      admit.    
+Admitted.
+
+
+Lemma body_findRecordIndex: semax_body Vprog Gprog f_findRecordIndex findRecordIndex_spec.
+Proof.
+  start_function.
+Admitted.
+
