verif/verif_newcursor.v
@@ -14,8 +14,9 @@ Require Import FunInd.
 Require Import btrees.
 Require Import btrees_sep.
 Require Import btrees_spec.
+Require Import verif_movetofirst.
 
-Lemma upd_repeat: forall X i (a:X) b m, 0 <= i -> (Z.to_nat i <= m)%nat -> m=MaxTreeDepth ->  
+Lemma upd_repeat: forall X i (a:X) b m, 0 <= i -> (Z.to_nat i < m)%nat -> m=MaxTreeDepth ->  
     upd_Znth i (list_repeat (Z.to_nat i) a ++ list_repeat (m - Z.to_nat i) b) a =
     (list_repeat (Z.to_nat (i+1)) a) ++ list_repeat (m - Z.to_nat (i+1)) b.
 Proof.
@@ -27,44 +28,92 @@ Proof.
   rewrite Zlength_list_repeat by auto.
   simpl. assert (i-i=0). omega. rewrite H3.
   unfold upd_Znth. simpl.
-  assert ((m - (Z.to_nat i))%nat = Z.to_nat (20-i)).
-  admit. rewrite H4.
+  assert ((m - (Z.to_nat i))%nat = Z.to_nat (20-i)). admit.
+  assert ((m - (Z.to_nat i + 1))%nat = Z.to_nat (20-i-1)). admit.
+  rewrite H4. rewrite H5.
   rewrite sublist_list_repeat.
-  admit.
-  omega. admit.                  (* false! *)
-  rewrite Zlength_list_repeat. split. omega. admit. auto.  
+  rewrite Zlength_list_repeat. rewrite <- app_assoc. auto.
+  admit.                        (* OK *)
+  omega.
+  rewrite Zlength_list_repeat. split; auto.
+  admit.                        (* OK *)
+  apply Z.le_refl.
+  admit.                        (* OK *)
+  rewrite Zlength_list_repeat. split. apply Z.le_refl.
+  assert ((m - (Z.to_nat i))%nat = Z.to_nat (20-i)). admit.
+  rewrite H3. admit.              (* OK *)
+  auto.
 Admitted.
 
 Lemma body_NewCursor: semax_body Vprog Gprog f_RL_NewCursor RL_NewCursor_spec.
 Proof.
   start_function.
+  destruct r as [[[root numRec] depth] prel].
+  pose (r:=(root,numRec,depth,prel)). fold r.
   forward_if (PROP() LOCAL(temp _relation p) SEP(relation_rep r p))%assert.
   - forward. auto.
   - subst p.
     assert_PROP(False).
-    entailer!. inv H0.
+    entailer!. contradiction.
   - forward_call tcursor.
     + split. unfold sizeof. simpl. rep_omega. split; auto.
     + Intros vret.
-      forward_if ((PROP (vret<>nullval)
-                        LOCAL (temp _cursor vret; temp _relation p)
-                        SEP (if eq_dec vret nullval
-                             then emp
-                             else malloc_token Tsh tcursor vret * data_at_ Tsh tcursor vret; 
-                             relation_rep r p))).
+      forward_if.
       * if_tac; entailer!.
       * rewrite if_true; auto.
-        forward. Exists nullval. entailer!.
-      * forward. rewrite if_false; auto. entailer!.
-      * Intros. rewrite if_false; auto. Intros.
-        forward.                  (* cursor->relation=relation *)
-        forward.                  (* cursor->level=0 *)
-        unfold relation_rep. destruct r. destruct p0. destruct p0. Intros proot.
+        forward. Exists nullval. Exists p'. entailer!.
+      * rewrite if_false; auto. Intros.
+        forward.                (* skip *)
+        forward.                (* cursor->relation=relation *)
+        forward.                (* cursor->level=0 *)
+        unfold relation_rep. unfold r. Intros proot.
         forward.                  (* t'3=relation->root *)
         simpl. entailer!. unfold local. unfold lift1. entailer!.
         admit.
-        (* forward_call to MoveToFirst *)
-        admit.
+{       forward_call(r,prel,empty_cursor,vret,root,(getval root)).
+        - entailer!.
+        - unfold relation_rep. unfold r. Exists proot. entailer!.
+          change_compspecs CompSpecs. cancel.
+          unfold cursor_rep.
+          destruct (default_val tcursor) eqn:DEF.
+          unfold_data_at 1%nat.
+          destruct c eqn:HC.
+          Exists (snd c0). Exists (fst c0). unfold empty_cursor. simpl.
+          change_compspecs CompSpecs. cancel.
+        - split; try split; try split.
+          + unfold empty_cursor. unfold Zlength. simpl. omega.
+          + unfold empty_cursor. unfold Zlength. simpl. rewrite MTD_eq. simpl. omega.
+          + auto.
+          + fold r in H0. auto.
+        - unfold cursor_rep. Intros anc_end. Intros idx_end. unfold r.
+          forward.              (* t'2=cursor->level *)
+          forward.              (* i=t'2+1 *)
+          + entailer!. unfold empty_cursor.
+            admit.              (* after moveToFirst, size of cursor in range *)
+          + (* gather_SEP 1 2 3 4 5 6. *)
+            (* replace_SEP 0 (cursor_rep (moveToFirst root empty_cursor (length empty_cursor)) r vret). *)
+            (* entailer!. unfold cursor_rep. Exists anc_end. Exists idx_end. entailer!. *)
+            autorewrite with norm.
+{ (* forward_loop ( *)
+  (*    EX i:Z,                   *)
+  (*    PROP ( i<=20 ) *)
+  (*    LOCAL (temp _i (Vint(Int.repr i)); *)
+  (*    temp _t'2 (Vint (Int.repr (Zlength (moveToFirst root empty_cursor (length empty_cursor)) - 1))); *)
+  (*    temp _t'3 proot; temp _cursor vret; temp _relation p) *)
+  (*    SEP (relation_rep (root, numRec, depth, prel) prel; malloc_token Tsh tcursor vret; *)
+  (*    field_at Tsh tcursor [StructField _relation] prel vret; *)
+  (*    field_at Tsh tcursor [StructField _level] *)
+  (*      (Vint (Int.repr (Zlength (moveToFirst root empty_cursor (length empty_cursor)) - 1))) vret; *)
+  (*    field_at Tsh tcursor [StructField _ancestorsIdx] *)
+  (*      (rev *)
+  (*         (map (fun x : node val * index.index => rep_index (snd x)) *)
+  (*            (moveToFirst root empty_cursor (length empty_cursor))) ++ idx_end) vret; *)
+  (*    field_at Tsh tcursor [StructField _ancestors] *)
+  (*      (rev (map getval (map fst (moveToFirst root empty_cursor (length empty_cursor)))) ++ anc_end) *)
+  (*      vret; emp)%assert). *)
+  (* should we do the loop ?  *)
+  admit.
+          
 Admitted.
 
 
