verif/verif_relation_mem.v
@@ -11,12 +11,16 @@ Require Import VST.msl.iter_sepcon.
 Require Import VST.floyd.reassoc_seq.
 Require Import VST.floyd.field_at_wand.
 Require Import FunInd.
+
+Require Import index.
 Require Import btrees.
 Require Import btrees_sep.
 Require Import btrees_spec.
+Require Import verif_findindex.
 Require Import verif_entryindex.
 Require Import verif_currnode.
 Require Import verif_isvalid.
+Require Import verif_movetofirst.
 Require Import verif_newnode.
 Require Import verif_newrel.
 Require Import verif_newcursor.
